QuickSortInLean/Sorted.lean
@@ -12,56 +12,52 @@ def sorted [Ord α] (arr : Array α) : Prop :=
   ∀i j : Fin arr.size, i ≤ j → (compare arr[i] arr[j]).isLE
 
 structure partitionImpl.LoopInvariant {α : Type} [Ord α] {n : Nat}
-  (arr : Vec α n) (first i j last : Nat)
-  (fn : first < n) (jn : j < n) (ln : last < n) : Prop where
+  (arr : Vec α n) (first i j last : Fin n) : Prop where
   intro ::
-  inv₁ : ∀k, i < k → (kj : k < j) → arr[k]'(Nat.lt_trans kj jn) <o arr[first]
-  inv₂ : ∀k, j < k → (kl : k ≤ last) → ¬arr[k]'(Nat.lt_of_le_of_lt kl ln) <o arr[first]
+  inv₁ : ∀k, i < k → (kj : k < j) → arr[k] <o arr[first]
+  inv₂ : ∀k, j < k → (kl : k ≤ last) → ¬arr[k] <o arr[first]
   inv₃ : i < j → arr[j] <o arr[first]
 
--- TODO: derivableなinequalityをdefault argumentで用意する
 theorem partitionImpl.loop_invariant {α : Type} [Ord α] {n : Nat}
-  (arr : Vec α n) (first i j last : Nat)
-  (fi : first ≤ i) (ij : i ≤ j) (fn : first < n) (jn : j < n) (ln : last < n)
-  (inv : LoopInvariant arr first i j last fn jn ln)
+  (arr : Vec α n) (first i j last : Fin n)
+  (fi : first ≤ i) (ij : i ≤ j)
+  (inv : LoopInvariant arr first i j last)
   (result : { mid : Nat // first ≤ mid ∧ mid ≤ j } × Vec α n)
-  (eq : partitionImpl arr first i j fi ij jn = result) :
-  LoopInvariant result.2 first first result.1 last fn (Nat.lt_of_le_of_lt result.1.property.2 jn) ln := by
-
-  induction arr, first, i, j, fi, ij, jn using partitionImpl.induct with
-  | base arr first i j fi _ _ _ _ h =>
-    have : i = first := Nat.le_antisymm (Nat.le_of_not_lt h) fi
-    rw [←eq]
-    simp [*, this ▸ inv]
-  | step_lt arr first i j _ _ jn _ _ fi _ lt _ ih =>
-    rw [←eq]
+  (eq : partitionImpl arr first i j fi ij = result) :
+  LoopInvariant result.2 first first ⟨result.1.val, Nat.lt_of_le_of_lt result.1.property.2 j.isLt⟩ last := by
+  induction arr, first, i, j, fi, ij using partitionImpl.induct with
+  | base arr first i j fi _ h =>
+    revert result
     simp [*]
-
-    have inv : LoopInvariant arr first (i - 1) j last fn jn ln := by
+    have : i = first := Fin.eq_of_val_eq (Nat.le_antisymm (Nat.le_of_not_lt h) fi)
+    exact this ▸ inv
+  | step_lt arr first i j _ _ fi _ lt _ ih =>
+    have inv : LoopInvariant arr first ⟨i.val - 1, Fin.sub_isLt⟩ j last := by
       apply LoopInvariant.intro
       . intro k ik kj
-        have ik : i ≤ k := by
+        have ik : i.val ≤ k.val := by
           rw [←Nat.sub_add_cancel (Nat.zero_lt_of_lt fi)]
           exact ik
         cases Nat.eq_or_lt_of_le ik with
         | inl ik =>
-          simp [ik] at lt
+          simp [Fin.eq_of_val_eq ik] at lt
           exact lt
         | inr ik => exact inv.1 k ik kj
       . exact inv.2
       . intro ij
-        have ij : i ≤ j := by
+        have ij : i.val ≤ j.val := by
           rw [←Nat.sub_add_cancel (Nat.zero_lt_of_lt fi)]
           exact ij
         cases Nat.eq_or_lt_of_le ij with
         | inl ij =>
-          simp [ij.symm]
+          simp [Fin.eq_of_val_eq ij.symm]
           assumption
         | inr ij => exact inv.3 ij
 
-    exact ih (by assumption) inv (partitionImpl arr first (i - 1) j (by assumption) (by assumption) (by assumption)) (by rfl)
-  | step_ge arr first i j _ ij jn _ _ fi _ _ _ _ ih =>
-    let swapped := arr.swap ⟨i, by assumption⟩ ⟨j, by assumption⟩
+    simp [*] at eq
+    apply ih inv result eq
+  | step_ge arr first i j _ ij fi _ _ _ ih =>
+    let swapped := arr.swap i j
     have sf : swapped[first] = arr[first] := by
       apply Vec.get_swap_neq
       . apply Fin.ne_of_val_ne
@@ -69,24 +65,23 @@ theorem partitionImpl.loop_invariant {α : Type} [Ord α] {n : Nat}
       . apply Fin.ne_of_val_ne
         exact Nat.ne_of_lt (Nat.lt_of_lt_of_le fi ij)
 
-    let result := partitionImpl swapped first (i - 1) (j - 1) (by assumption) (by assumption) (by assumption)
-    rw [←eq]
+    let result := partitionImpl swapped first ⟨i - 1, Fin.sub_isLt⟩ ⟨j - 1, Fin.sub_isLt⟩ (by assumption) (by assumption)
+    subst eq
     simp [*]
 
-    have inv : LoopInvariant swapped first (i - 1) (j - 1) last fn (Nat.lt_of_le_of_lt (Nat.sub_le ..) jn) ln := by
+    have inv : LoopInvariant swapped first ⟨i - 1, Fin.sub_isLt⟩ ⟨j - 1, Fin.sub_isLt⟩ last := by
       apply LoopInvariant.intro
       . intro k ik kj
-        have : k < n := Nat.lt_trans kj (by assumption)
-        have ik : i ≤ k := by
+        have ik : i.val ≤ k.val := by
           rw [←Nat.sub_add_cancel (Nat.zero_lt_of_lt fi)]
           exact ik
         cases Nat.eq_or_lt_of_le ik with
         | inl ik =>
           have : swapped[k] = arr[j] := by
-            simp [ik.symm]
+            simp [Fin.eq_of_val_eq ik.symm]
             apply Vec.get_swap_left
           rw [this, sf]
-          exact inv.3 (Nat.lt_of_lt_of_le (ik.symm ▸ kj) (Nat.sub_le ..))
+          exact inv.3 (Nat.lt_of_lt_of_le (Fin.eq_of_val_eq ik.symm ▸ kj) (Nat.sub_le ..))
         | inr ik =>
           have kj : k < j := (Nat.lt_of_lt_of_le kj (Nat.sub_le ..))
           have : swapped[k] = arr[k] := by
@@ -98,14 +93,13 @@ theorem partitionImpl.loop_invariant {α : Type} [Ord α] {n : Nat}
           rw [this, sf]
           exact inv.1 k ik kj
       . intro k jk kl
-        have : k < n := Nat.lt_of_le_of_lt kl (by assumption)
-        have jk : j ≤ k := by
+        have jk : j.val ≤ k.val := by
           rw [←Nat.sub_add_cancel (Nat.zero_lt_of_lt (Nat.zero_lt_of_lt (Nat.lt_of_lt_of_le fi ij)))]
           exact jk
         cases Nat.eq_or_lt_of_le jk with
         | inl jk =>
           have : swapped[k] = arr[i] := by
-            simp [jk.symm]
+            simp [Fin.eq_of_val_eq jk.symm]
             apply Vec.get_swap_right
           rw [this, sf]
           assumption
@@ -119,41 +113,41 @@ theorem partitionImpl.loop_invariant {α : Type} [Ord α] {n : Nat}
           rw [this, sf]
           exact inv.2 k jk kl
       . intro ij
-        have : j - 1 < j := by
-          show j - 1 + 1 ≤ j
+        have : j.val - 1 < j.val := by
+          show j.val - 1 + 1 ≤ j.val
           rw [Nat.sub_add_cancel (Nat.zero_lt_of_lt (Nat.lt_of_lt_of_le fi (by assumption)))]
           apply Nat.le_refl
-        have ij : i ≤ j - 1 := by
+        have ij : i.val ≤ j.val - 1 := by
           rw [←Nat.sub_add_cancel (Nat.zero_lt_of_lt fi)]
           exact ij
         cases Nat.eq_or_lt_of_le ij with
         | inl ij =>
-          have : swapped[j - 1] = arr[j] := by
+          have : swapped[Fin.mk (j - 1) Fin.sub_isLt] = arr[j] := by
             simp [ij.symm]
             apply Vec.get_swap_left
           rw [this, sf]
-          have : i < j := Nat.lt_of_le_of_lt (by assumption : i ≤ j - 1) (by assumption)
+          have : i < j := Nat.lt_of_le_of_lt (by assumption : i.val ≤ j.val - 1) (by assumption)
           exact inv.3 this
         | inr ij =>
-          have : swapped[j - 1] = arr[j - 1] := by
+          have : swapped[Fin.mk (j - 1) Fin.sub_isLt] = arr[Fin.mk (j - 1) Fin.sub_isLt] := by
             apply Vec.get_swap_neq
             . apply Fin.ne_of_val_ne
               exact Nat.ne_of_gt ij
             . apply Fin.ne_of_val_ne
               exact Nat.ne_of_lt (by assumption)
           rw [this, sf]
-          apply inv.1 (j - 1) ij (by assumption)
+          apply inv.1 ⟨j - 1, Fin.sub_isLt⟩ ij (by assumption)
 
-    exact ih (by assumption) inv result (by rfl)
+    exact ih inv result (by rfl)
 
 theorem partitionImpl.first_eq {α : Type} [Ord α] {n : Nat}
-  (arr : Vec α n) (first i j : Nat)
-  (fi : first ≤ i) (ij : i ≤ j) (jn : j < n) (fn : first < n := Nat.lt_of_le_of_lt (Nat.le_trans fi ij) jn):
-  (partitionImpl arr first i j fi ij jn).2[first] = arr[first] := by
-  induction arr, first, i, j, fi, ij, jn using partitionImpl.induct with
+  (arr : Vec α n) (first i j : Fin n)
+  (fi : first ≤ i) (ij : i ≤ j) :
+  (partitionImpl arr first i j fi ij).2[first] = arr[first] := by
+  induction arr, first, i, j, fi, ij using partitionImpl.induct with
   | base => simp [*]
   | step_lt => simp [*]
-  | step_ge arr first i j _ ij _ _ _ fi =>
+  | step_ge arr first i j _ ij fi =>
     simp [*]
     have fj : first < j := Nat.lt_of_lt_of_le fi ij
     apply Vec.get_swap_neq
@@ -163,20 +157,20 @@ theorem partitionImpl.first_eq {α : Type} [Ord α] {n : Nat}
       exact Nat.ne_of_lt fj
 
 theorem partition.partition {α : Type} [Ord α] {n : Nat}
-  (arr : Vec α n) (first last : Nat)
-  (fl : first ≤ last) (ln : last < n)
+  (arr : Vec α n) (first last : Fin n) (fl : first ≤ last)
   (result : { mid : Nat // first ≤ mid ∧ mid ≤ last } × Vec α n)
-  (eq : partition arr first last fl ln = result) :
-  (∀k : Nat, first ≤ k → (km : k < result.1) →
-    result.2[k]'(Nat.lt_trans km (Nat.lt_of_le_of_lt result.1.property.2 ln)) <o arr[first]'(Nat.lt_of_le_of_lt fl ln)) ∧
-  (result.2[result.1.val]'(Nat.lt_of_le_of_lt result.1.property.2 ln) = arr[first]'(Nat.lt_of_le_of_lt fl ln)) ∧
-  (∀k : Nat, result.1 < k → (kl : k ≤ last) →
-    ¬result.2[k]'(Nat.lt_of_le_of_lt kl ln) <o arr[first]'(Nat.lt_of_le_of_lt fl ln)) := by
+  (eq : partition arr first last fl = result) :
+  (∀k : Fin n, first ≤ k → (km : k.val < result.1.val) →
+    result.2[k] <o arr[first]) ∧
+  (result.2[result.1.val]'(Nat.lt_of_le_of_lt result.1.property.2 last.isLt) = arr[first]) ∧
+  (∀k : Fin n, result.1.val < k.val → (kl : k ≤ last) →
+    ¬result.2[k] <o arr[first]) := by
 
-  let afterLoop := partitionImpl arr first last last fl .refl ln
+  let afterLoop := partitionImpl arr first last last fl (Nat.le_refl _)
   let mid := afterLoop.1
   let arr' := afterLoop.2
-  let swapped := arr'.swap ⟨first, Nat.lt_of_le_of_lt fl ln⟩ ⟨mid, Nat.lt_of_le_of_lt mid.property.2 ln⟩
+  have : mid < n := Nat.lt_of_le_of_lt mid.property.2 last.isLt
+  let swapped := arr'.swap first ⟨mid, by assumption⟩
   have : result.1 = mid := by
     rw [←eq]
     unfold partition
@@ -185,13 +179,11 @@ theorem partition.partition {α : Type} [Ord α] {n : Nat}
     rw [←eq]
     unfold partition
     simp [afterLoop, dbgTraceIfShared]
-  have : first < n := Nat.lt_of_le_of_lt fl ln
-  have : mid < n := Nat.lt_of_le_of_lt mid.property.2 ln
 
   have first_eq : arr'[first] = arr[first] := by
     apply partitionImpl.first_eq
 
-  let inv₀ : partitionImpl.LoopInvariant arr first last last last (by assumption) ln ln := by
+  let inv₀ : partitionImpl.LoopInvariant arr first last last last := by
     apply partitionImpl.LoopInvariant.intro
     . intro k lk kl
       exact (Nat.lt_irrefl k (Nat.lt_trans kl lk)).elim
@@ -199,21 +191,18 @@ theorem partition.partition {α : Type} [Ord α] {n : Nat}
       exact (Nat.lt_irrefl k (Nat.lt_of_le_of_lt kl lk)).elim
     . intro ll
       exact (Nat.lt_irrefl last ll).elim
-  let inv := partitionImpl.loop_invariant arr first last last last fl .refl (by assumption) ln ln inv₀ afterLoop (by rfl)
-  let ⟨a, b, c⟩ := inv
+  let inv := partitionImpl.loop_invariant arr first last last last fl (Nat.le_refl _) inv₀ afterLoop (by rfl)
 
-  have p₁ (k : Nat) (fk : first ≤ k) (km : k < mid) : swapped[k]'(Nat.lt_trans km (Nat.lt_of_le_of_lt mid.property.2 ln)) <o arr[first] := by
-    have : k < n := Nat.lt_trans km (by assumption)
-
+  have p₁ (k : Fin n) (fk : first ≤ k) (km : k.val < mid) : swapped[k] <o arr[first] := by
     cases Nat.eq_or_lt_of_le fk with
     | inl fk =>
       have : swapped[k] = swapped[first] := by
-        simp [fk]
+        simp [Fin.eq_of_val_eq fk]
       rw [this]
       have : swapped[first] = arr'[mid.val] := by
         apply Vec.get_swap_left
       rw [this, ←first_eq]
-      exact inv.3 (fk ▸ km)
+      exact inv.3 (Fin.eq_of_val_eq fk ▸ km)
     | inr fk =>
       have : swapped[k] = arr'[k] := by
         apply Vec.get_swap_neq
@@ -230,8 +219,7 @@ theorem partition.partition {α : Type} [Ord α] {n : Nat}
     rw [this]
     assumption
 
-  have p₃ (k : Nat) (mk : mid < k) (kl : k ≤ last) : ¬swapped[k]'(Nat.lt_of_le_of_lt kl ln) <o arr[first] := by
-    have : k < n := Nat.lt_of_le_of_lt kl ln
+  have p₃ (k : Fin n) (mk : mid < k.val) (kl : k ≤ last) : ¬swapped[k] <o arr[first] := by
     have : swapped[k] = arr'[k] := by
       apply Vec.get_swap_neq
       . apply Fin.ne_of_val_ne
@@ -263,51 +251,47 @@ def Nat.range_split (i j x : Nat) (ij : i ≤ j) : Nat.RangeSplit i j x ij :=
     | isFalse ix => .split (Nat.le_of_not_lt ix) (Nat.le_of_lt jx)
 
 theorem quickSortImpl.get_lt {α : Type} [Ord α] {n : Nat}
-  (arr : Vec α n) (first last : Nat) (ln : last < n)
+  (arr : Vec α n) (first : Nat) (last : Fin n)
   (k : Fin n) (lt : k < first) :
-  (quickSortImpl arr first last ln)[k] = arr[k] := by
-  let p := quickSortImpl_permuted arr first last ln
+  (quickSortImpl arr first last)[k] = arr[k] := by
+  let p := quickSortImpl_permuted arr first last
   exact p.get_lt lt
 
 theorem quickSortImpl.get_gt {α : Type} [Ord α] {n : Nat}
-  (arr : Vec α n) (first last : Nat) (ln : last < n)
+  (arr : Vec α n) (first : Nat) (last : Fin n)
   (k : Fin n) (gt : k > last) :
-  (quickSortImpl arr first last ln)[k] = arr[k] := by
-  let p := quickSortImpl_permuted arr first last ln
+  (quickSortImpl arr first last)[k] = arr[k] := by
+  let p := quickSortImpl_permuted arr first last
   exact p.get_gt gt
 
 theorem quickSortImpl_sortedRange {α : Type} [Order α] {n : Nat}
-  (arr : Vec α n) (first last : Nat) (ln : last < n) :
-  sortedRange (quickSortImpl arr first last ln) first last := by
-  induction arr, first, last, ln using quickSortImpl.induct with
-  | base arr first last ln h =>
+  (arr : Vec α n) (first : Nat) (last : Fin n) :
+  sortedRange (quickSortImpl arr first last) first last := by
+  induction arr, first, last using quickSortImpl.induct with
+  | base arr first last h =>
     simp [*]
     intro i j fi ij jl
     have : first = last := Nat.le_antisymm (Nat.le_trans (Nat.le_trans fi ij) jl) (Nat.le_of_not_gt h)
     subst this
-    have hi : i = first := Nat.le_antisymm (Nat.le_trans ij jl) fi
-    have hj : j = first := Nat.le_antisymm jl (Nat.le_trans fi ij)
-    have : i = j := by
-      apply Fin.eq_of_val_eq
-      simp [hi, hj]
+    have : i = last := Fin.eq_of_val_eq (Nat.le_antisymm (Nat.le_trans ij jl) fi)
+    subst this
+    have : i = j := Fin.eq_of_val_eq (Nat.le_antisymm ij jl)
     subst this
     apply Order.refl
-  | step arr first last ln lt parted eq ih₁ ih₂ =>
+  | step arr first last lt parted eq _ ih₁ ih₂ =>
+    have : first < n := Nat.lt_trans lt last.isLt
     simp [*]
     intro i j fi ij jl
 
     let mid := parted.1
-    have : first < n := Nat.lt_trans lt ln
-    have mn : mid.val < n := Nat.lt_of_le_of_lt mid.property.2 ln
-    have : mid.val - 1 < n := Nat.lt_of_le_of_lt (Nat.sub_le ..) mn
-    let sorted := quickSortImpl (quickSortImpl parted.snd first (parted.fst.val - 1) (by assumption))
-      (parted.fst.val + 1) last ln
+    have mn : mid.val < n := Nat.lt_of_le_of_lt mid.property.2 last.isLt
+    let sorted := quickSortImpl (quickSortImpl parted.snd first ⟨mid.val - 1, by assumption⟩) (mid.val + 1) last
 
-    let ⟨l, m, r⟩ := partition.partition arr first last (Nat.le_of_lt lt) ln parted eq
+    let ⟨l, m, r⟩ := partition.partition arr ⟨first, by assumption⟩ last (Nat.le_of_lt lt) parted eq
 
     have getL (k : Fin n) (fk : first ≤ k) (km : k < mid.val) : sorted[k] <o arr[first] := by
       rw [quickSortImpl.get_lt (lt := (Nat.lt_trans km (Nat.lt_succ_self ..)))]
-      let p := quickSortImpl_permuted parted.2 first (mid.val - 1) (by assumption)
+      let p := quickSortImpl_permuted parted.2 first ⟨mid.val - 1, by assumption⟩
       let ⟨k', ⟨index, fk', km'⟩⟩ := permuted_map_index_in_range_inv p k fk (Nat.le_sub_one_of_lt km)
       let inv := index ▸ permuted_map_index p k'
       rw [←inv]
@@ -322,19 +306,21 @@ theorem quickSortImpl_sortedRange {α : Type} [Order α] {n : Nat}
       rw [quickSortImpl.get_lt (k := mid') (lt := Nat.lt_succ_self ..)]
       cases Nat.eq_zero_or_pos mid.val with
       | inl zero =>
-        rw [←m]
-        simp [zero]
-        rfl
+        simp [zero] at *
+        exact m
       | inr pos =>
         rw [quickSortImpl.get_gt (k := mid') (gt := Nat.sub_lt_self (by decide) (Nat.zero_lt_of_lt pos))]
         exact m
 
     have getR (k : Fin n) (mk : mid.val < k) (kl : k ≤ last) : ¬sorted[k] <o arr[first] := by
-      let p := quickSortImpl_permuted (quickSortImpl parted.snd first (parted.fst.val - 1) (by assumption)) (mid.val + 1) last ln
+      let p := quickSortImpl_permuted (quickSortImpl parted.snd first ⟨mid.val - 1, by assumption⟩) (mid.val + 1) last
       let ⟨k', ⟨index, mk', kl'⟩⟩ := permuted_map_index_in_range_inv p k mk kl
       let inv := index ▸ permuted_map_index p k'
       rw [←inv]
-      rw [quickSortImpl.get_gt (gt := Nat.lt_of_le_of_lt (Nat.sub_le ..) mk')]
+      have : (⟨mid.val - 1, by assumption⟩ : Fin n).val ≤ mid.val := by
+        simp
+        exact (Nat.sub_le ..)
+      rw [quickSortImpl.get_gt (gt := Nat.lt_of_le_of_lt this mk')]
       apply r k' mk' kl'
 
     have getLM (k : Fin n) (fk : first ≤ k) (km : k ≤ mid.val) : sorted[k] ≤o arr[first] := by
