QuickSortInLean/Induction.lean
@@ -1,124 +1,118 @@
 import QuickSortInLean.QuickSort
 
 theorem partitionImpl.induct {α : Type} [Ord α] {n : Nat}
-  (motive : (arr : Vec α n) → (first i j : Nat) → (fi : first ≤ i) → (ij : i ≤ j) → (jn : j < n) → Sort u)
-  (arr : Vec α n) (first i j : Nat)
-  (fi : first ≤ i) (ij : i ≤ j) (jn : j < n)
-  (base : ∀arr first i j fi ij jn (_ : i < n) (_ : first < n) (_ : ¬first < i), motive arr first i j fi ij jn)
-  (step_lt : ∀arr first i j fi ij jn
-    (_ : i < n) (_ : first < n) (_ : first < i) (_ : first ≤ i - 1) (_ : arr[i] <o arr[first]) (_ : i - 1 ≤ j)
-    (ih : motive arr first (i - 1) j (by assumption) (by assumption) jn),
-    motive arr first i j fi ij jn)
-  (step_ge : ∀arr first i j fi ij jn
-    (_ : i < n) (_ : first < n) (_ : first < i) (_ : first ≤ i - 1) (_ : ¬arr[i] <o arr[first]) (_ : i - 1 ≤ j - 1) (_ : j - 1 < n)
-    (ih : motive (arr.swap ⟨i, by assumption⟩ ⟨j, jn⟩) first (i - 1) (j - 1) (by assumption) (by assumption) (by assumption)),
-    motive arr first i j fi ij jn)
-  : motive arr first i j fi ij jn := by
-  have : i < n := Nat.lt_of_le_of_lt ij jn
-  have : first < n := Nat.lt_of_le_of_lt fi this
+  (motive : (arr : Vec α n) → (first i j : Fin n) → (fi : first ≤ i) → (ij : i ≤ j) → Sort u)
+  (arr : Vec α n) (first i j : Fin n)
+  (fi : first ≤ i) (ij : i ≤ j)
+  (base : ∀arr first i j fi ij (_ : ¬first < i), motive arr first i j fi ij)
+  (step_lt : ∀arr (first i j : Fin n) fi ij
+    (_ : first < i) (_ : first ≤ i.val - 1) (_ : arr[i] <o arr[first]) (_ : i.val - 1 ≤ j)
+    (ih : motive arr first ⟨i.val - 1, Fin.sub_isLt⟩ j (by assumption) (by assumption)),
+    motive arr first i j fi ij)
+  (step_ge : ∀arr (first i j : Fin n) fi ij
+    (_ : first < i) (_ : first ≤ i.val - 1) (_ : ¬arr[i] <o arr[first]) (_ : i.val - 1 ≤ j.val - 1)
+    (ih : motive (arr.swap i j) first ⟨i - 1, Fin.sub_isLt⟩ ⟨j - 1, Fin.sub_isLt⟩ (by assumption) (by assumption)),
+    motive arr first i j fi ij)
+  : motive arr first i j fi ij := by
   if h : first < i then
-    have : first ≤ i - 1 := Nat.le_sub_of_lt h
+    have : first ≤ i.val - 1 := Nat.le_sub_one_of_lt h
     if _ : arr[i] <o arr[first] then
-      have : i - 1 ≤ j := Nat.le_trans (Nat.sub_le ..) ij
-      apply step_lt arr first i j fi ij jn
-        (by assumption) (by assumption) h (by assumption) (by assumption)
+      have : i.val - 1 ≤ j := Nat.le_trans (Nat.sub_le ..) ij
+      apply step_lt arr first i j fi ij h (by assumption) (by assumption)
       apply partitionImpl.induct motive
-        arr first (i - 1) j
-        (by assumption) (by assumption) jn
+        arr first ⟨i - 1, Fin.sub_isLt⟩ j
+        (by assumption) (by assumption)
         base step_lt step_ge
     else
-      have : i - 1 ≤ j - 1 := Nat.sub_le_sub_right ij 1
-      have : j - 1 < n := Nat.lt_of_le_of_lt (Nat.sub_le ..) jn
-      let arr' := arr.swap ⟨i, by assumption⟩ ⟨j, jn⟩
-      apply step_ge arr first i j fi ij jn
-        (by assumption) (by assumption) h (by assumption) (by assumption) (by assumption) (by assumption)
+      have : i.val - 1 ≤ j.val - 1 := Nat.sub_le_sub_right ij 1
+      let arr' := arr.swap i j
+      apply step_ge arr first i j fi ij h (by assumption) (by assumption) (by assumption)
       apply partitionImpl.induct motive
-        arr' first (i - 1) (j - 1)
-        (by assumption) (by assumption) (by assumption)
+        arr' first ⟨i - 1, Fin.sub_isLt⟩ ⟨j - 1, Fin.sub_isLt⟩
+        (by assumption) (by assumption)
         base step_lt step_ge
   else
-    apply base arr first i j fi ij jn (by assumption) (by assumption) h
+    apply base arr first i j fi ij h
+termination_by _ => i.val
 
 @[simp]
 theorem partitionImpl.simp_base {α : Type} [Ord α]
-  {n : Nat} {arr : Vec α n} {first i j : Nat}
-  {fi : first ≤ i} {ij : i ≤ j} {jn : j < n}
+  {n : Nat} {arr : Vec α n} {first i j : Fin n}
+  {fi : first ≤ i} {ij : i ≤ j}
   (h : ¬first < i) :
-  partitionImpl arr first i j fi ij jn =
+  partitionImpl arr first i j fi ij =
   (⟨j, ⟨Nat.le_trans (by assumption) ij, by simp⟩⟩, arr) := by
   unfold partitionImpl
   simp [*, dbgTraceIfShared]
 
 @[simp]
 theorem partitionImpl.simp_step_lt {α : Type} [Ord α]
-  {n : Nat} {arr : Vec α n} {first i j : Nat}
-  {fi : first ≤ i} {ij : i ≤ j} {jn : j < n}
-  (h : first < i) (_ : ltOfOrd.lt (arr[i]'(Nat.lt_of_le_of_lt ij jn)) (arr[first]'(Nat.lt_of_le_of_lt fi (Nat.lt_of_le_of_lt ij jn)))) :
-  partitionImpl arr first i j fi ij jn = partitionImpl arr first (i - 1) j (Nat.le_sub_of_lt h) (Nat.le_trans (Nat.sub_le ..) ij) jn := by
+  {n : Nat} {arr : Vec α n} {first i j : Fin n}
+  {fi : first ≤ i} {ij : i ≤ j}
+  (h : first < i) (_ : arr[i] <o arr[first]) :
+  partitionImpl arr first i j fi ij = partitionImpl arr first ⟨i - 1, Fin.sub_isLt⟩ j (Nat.le_sub_one_of_lt h) (Nat.le_trans (Nat.sub_le ..) ij) := by
   rw [partitionImpl]
   simp [*]
 
 @[simp]
 theorem partitionImpl.simp_step_ge {α : Type} [Ord α]
-  {n : Nat} {arr : Vec α n} {first i j : Nat}
-  {fi : first ≤ i} {ij : i ≤ j} {jn : j < n} (h : first < i) (_ : ¬arr[i]'(Nat.lt_of_le_of_lt ij jn) <o arr[first]'(Nat.lt_of_le_of_lt fi (Nat.lt_of_le_of_lt ij jn))) :
-  partitionImpl arr first i j fi ij jn =
-  match partitionImpl (arr.swap ⟨i, Nat.lt_of_le_of_lt ij jn⟩ ⟨j, jn⟩) first (i - 1) (j - 1)
-    (Nat.le_sub_of_lt h) (Nat.sub_le_sub_right ij 1) (Nat.lt_of_le_of_lt (Nat.sub_le ..) jn) with
+  {n : Nat} {arr : Vec α n} {first i j : Fin n}
+  {fi : first ≤ i} {ij : i ≤ j}
+  (h : first < i) (_ : ¬arr[i] <o arr[first]) :
+  partitionImpl arr first i j fi ij =
+  match partitionImpl (arr.swap i j) first ⟨i - 1, Fin.sub_isLt⟩ ⟨j - 1, Fin.sub_isLt⟩
+    (Nat.le_sub_one_of_lt h) (Nat.sub_le_sub_right ij 1) with
   | (⟨mid, hm⟩, arr) => (⟨mid, ⟨hm.1, Nat.le_trans hm.2 (Nat.sub_le ..)⟩⟩, arr) := by
   rw [partitionImpl]
   simp [*, dbgTraceIfShared]
 
 theorem quickSortImpl.induct {α : Type} [Ord α] {n : Nat}
-  (motive : (arr : Vec α n) → (first last : Nat) → (ln : last < n) → Sort u)
-  (arr : Vec α n) (first last : Nat) (ln : last < n)
-  (base : ∀arr first last ln (_ : ¬first < last), motive arr first last ln)
-  (step : ∀arr first last ln (lt : first < last)
-    (parted : { mid : Nat // first ≤ mid ∧ mid ≤ last } × Vec α n) (_ : partition arr first last (Nat.le_of_lt lt) ln = parted),
-    have : parted.1 - 1 < n := Nat.lt_of_le_of_lt (Nat.sub_le ..) (Nat.lt_of_le_of_lt parted.1.property.2 ln)
-    ∀(ih₁ : motive parted.2 first (parted.1 - 1) (by assumption))
-      (ih₂ : motive (quickSortImpl parted.2 first (parted.1 - 1) (by assumption)) (parted.1 + 1) last ln),
-    motive arr first last ln
+  (motive : (arr : Vec α n) → (first : Nat) → (last : Fin n) → Sort u)
+  (arr : Vec α n) (first : Nat) (last : Fin n)
+  (base : ∀arr (first : Nat) (last : Fin n) (_ : ¬first < last), motive arr first last)
+  (step : ∀arr (first : Nat) (last : Fin n) (lt : first < last)
+    (parted : { mid : Nat // first ≤ mid ∧ mid ≤ last } × Vec α n) (_ : partition arr ⟨first, Nat.lt_trans lt last.isLt⟩ last (Nat.le_of_lt lt) = parted)
+    (_ : parted.1 - 1 < n)
+    (ih₁ : motive parted.2 first ⟨parted.1 - 1, by assumption⟩)
+    (ih₂ : motive (quickSortImpl parted.2 first ⟨parted.1 - 1, by assumption⟩) (parted.1 + 1) last),
+    motive arr first last
   )
-  : motive arr first last ln := by
+  : motive arr first last := by
   if lt : first < last then
-    let parted := partition arr first last (Nat.le_of_lt lt) ln
+    let parted := partition arr ⟨first, Nat.lt_trans lt last.isLt⟩ last (Nat.le_of_lt lt)
     let mid := parted.1.val
     let hm := parted.1.property
-    have : mid - 1 < n := Nat.lt_of_le_of_lt (Nat.sub_le ..) (Nat.lt_of_le_of_lt hm.2 ln)
+    have : mid - 1 < n := Nat.lt_of_le_of_lt (Nat.sub_le ..) (Nat.lt_of_le_of_lt hm.2 last.isLt)
     -- Termination lemmas
     have : mid - 1 - first < last - first := quickSortImpl.termination_lemma first last lt hm.1 hm.2
     have : last - (mid + 1) < last - first := Nat.sub_lt_sub_left lt (Nat.lt_of_le_of_lt hm.1 (Nat.lt_succ_self ..))
 
-    apply step arr first last ln lt parted (Eq.refl parted)
+    apply step arr first last lt parted (Eq.refl parted) (by assumption)
     case ih₁ =>
-      show motive parted.2 first (mid - 1) (by assumption)
-      apply quickSortImpl.induct motive parted.2 first (mid - 1) (by assumption)
-        base step
+      apply quickSortImpl.induct motive parted.2 first ⟨mid - 1, by assumption⟩ base step
     case ih₂ =>
-      show motive (quickSortImpl parted.2 first (mid - 1) (by assumption)) (mid + 1) last ln
-      apply quickSortImpl.induct motive (quickSortImpl parted.2 first (mid - 1) (by assumption)) (mid + 1) last ln
+      apply quickSortImpl.induct motive (quickSortImpl parted.2 first ⟨mid - 1, by assumption⟩) (mid + 1) last
         base step
   else
-    apply base arr first last ln lt
+    apply base arr first last lt
 termination_by _ => last - first
 
 @[simp]
 theorem quickSortImpl.simp_base {α : Type} [Ord α]
-  {n : Nat} {arr : Vec α n} {first last : Nat} {ln : last < n}
+  {n : Nat} {arr : Vec α n} {first : Nat} {last : Fin n}
   (h : ¬first < last) :
-  quickSortImpl arr first last ln = arr := by
+  quickSortImpl arr first last = arr := by
   unfold quickSortImpl
   simp [*]
 
 @[simp]
 theorem quickSortImpl.simp_step {α : Type} [Ord α]
-  {n : Nat} {arr : Vec α n} {first last : Nat} {ln : last < n}
+  {n : Nat} {arr : Vec α n} {first : Nat} {last : Fin n}
   (lt : first < last) :
-  let parted := partition arr first last (Nat.le_of_lt lt) ln
+  let parted := partition arr ⟨first, Nat.lt_trans lt last.isLt⟩ last (Nat.le_of_lt lt)
   let mid := parted.1.val
   let hm := parted.1.property
-  have : mid - 1 < n := Nat.lt_of_le_of_lt (Nat.sub_le ..) (Nat.lt_of_le_of_lt hm.2 ln)
-  quickSortImpl arr first last ln = quickSortImpl (quickSortImpl parted.2 first (mid - 1) (by assumption)) (mid + 1) last ln := by
+  have : mid - 1 < n := Nat.lt_of_le_of_lt (Nat.sub_le ..) (Nat.lt_of_le_of_lt hm.2 last.isLt)
+  quickSortImpl arr first last = quickSortImpl (quickSortImpl parted.2 first ⟨mid - 1, by assumption⟩) (mid + 1) last := by
   rw [quickSortImpl]
   simp [*]
