QuickSortInLean/QuickSortPermutation.lean
@@ -3,42 +3,40 @@ import QuickSortInLean.QuickSort
 import QuickSortInLean.Induction
 
 theorem partitionImpl_permuted {α : Type} [Ord α]
-  {n : Nat} (arr : Vec α n) (first i j last : Nat)
-  (fi : first ≤ i) (ij : i ≤ j) (jl : j ≤ last) (jn : j < n) :
-  permuted n first last arr (partitionImpl arr first i j fi ij jn).2 := by
-  induction arr, first, i, j, fi, ij, jn using partitionImpl.induct with
+  {n : Nat} (arr : Vec α n) (first i j : Fin n)
+  (fi : first ≤ i) (ij : i ≤ j) :
+  permuted n first j arr (partitionImpl arr first i j fi ij).2 := by
+  induction arr, first, i, j, fi, ij using partitionImpl.induct with
   | base arr first i j fi ij jn =>
     simp [*]
     exact .refl
-  | step_lt arr first i j fi ij jn _ _ _ _ _ _ ih =>
+  | step_lt arr first i j fi ij _ _ _ _ ih =>
     simp [*]
-    exact ih jl
-  | step_ge arr first i j fi ij jn _ _ _ _ _ _ _ ih =>
+    exact ih
+  | step_ge arr first i j fi ij _ _ _ _ ih =>
     simp [*]
-    apply permuted.step ⟨i, by assumption⟩ ⟨j, jn⟩ fi ij jl (ih (Nat.le_trans (Nat.sub_le ..) jl))
+    apply permuted.step i j fi ij (Nat.le_refl _) (ih.cast_last (Nat.sub_le ..))
 
 theorem partition_permuted {α : Type} [Ord α]
-  {n : Nat} (arr : Vec α n) (first last : Nat)
-  (fl : first ≤ last) (ln : last < n) :
-  permuted n first last arr (partition arr first last fl ln).2 := by
-  let result := partition arr first last fl ln
+  {n : Nat} (arr : Vec α n) (first last : Fin n) (fl : first ≤ last) :
+  permuted n first last arr (partition arr first last fl).2 := by
+  let result := partition arr first last fl
   let mid := result.1
   simp [partition, dbgTraceIfShared]
-  let p := partitionImpl_permuted arr first last last last fl (Nat.le_refl _) (Nat.le_refl _) ln
+  let p := partitionImpl_permuted arr first last last fl (Nat.le_refl _)
   exact permuted.trans p
-    (.step ⟨first, Nat.lt_of_le_of_lt fl ln⟩ ⟨mid, Nat.lt_of_le_of_lt mid.property.2 ln⟩
-      (Nat.le_of_eq (Eq.refl _)) mid.property.1 mid.property.2 .refl)
+    (.step first ⟨mid, Nat.lt_of_le_of_lt mid.property.2 last.isLt⟩ (Nat.le_refl _) mid.property.1 mid.property.2 .refl)
 
 theorem quickSortImpl_permuted {α : Type} [Ord α]
-  {n : Nat} (arr : Vec α n) (first last : Nat) (ln : last < n) :
-  permuted n first last arr (quickSortImpl arr first last ln) := by
-  induction arr, first, last, ln using quickSortImpl.induct with
-  | base arr first last ln h =>
+  {n : Nat} (arr : Vec α n) (first : Nat) (last : Fin n) :
+  permuted n first last arr (quickSortImpl arr first last) := by
+  induction arr, first, last using quickSortImpl.induct with
+  | base arr first last h =>
     simp [*]
     exact .refl
-  | step arr first last ln lt parted eq ih₁ ih₂ =>
+  | step arr first last lt parted eq _ ih₁ ih₂ =>
     simp [*]
-    let p := partition_permuted arr first last (Nat.le_of_lt lt) ln
+    let p := partition_permuted arr ⟨first, Nat.lt_trans lt last.isLt⟩ last (Nat.le_of_lt lt)
     rw [eq] at p
     exact permuted.trans
       (permuted.trans p (ih₁.cast_last (Nat.le_trans (Nat.sub_le ..) parted.1.property.2)))
@@ -50,7 +48,7 @@ theorem quickSort'_permuted  {α : Type} [Ord α] {n : Nat} (arr : Vec α n) :
   match Nat.decLt 0 n with
   | isTrue h =>
     simp [h]
-    apply quickSortImpl_permuted arr
+    apply quickSortImpl_permuted arr 0 ⟨n - 1, Nat.sub_lt_self (by decide) (Nat.zero_lt_of_lt h)⟩
   | isFalse h =>
     simp [h]
     exact .refl
